More WIP on translation
The generic traversal looks rather nice (tho a datatype might work better?).
Simplifying the nested fixpoints is a pain (and intrinsically hard), so probably
better to avoid writing those.

dsub/operational.v
@@ -234,7 +234,6 @@ End to_subst_idsσ_is_id.
 Section translation.
   Definition stys := gmap stamp ty.
   Implicit Type g: stys.
-  Definition unstamp_vstamp g vs s := (default TNat (g !! s)).|[to_subst vs].
 
   Definition gdom {X} (g: gmap stamp X) := dom (gset stamp) g.
   Arguments gdom /.
@@ -253,6 +252,8 @@ Section translation.
     pose proof (fresh_stamp_strong g T) as [s []].
     exists s; split =>//=. by apply subseteq_dom.
   Qed.
+
+  Definition unstamp_vstamp g vs s := (from_option vty (vstamp vs s) (g !! s)).[to_subst vs].
   Arguments unstamp_vstamp /.
 
   Fixpoint unstamp_tm g (t: tm): tm :=
@@ -267,7 +268,7 @@ Section translation.
   unstamp_vl g (v: vl): vl :=
     let fix go (v: vl): vl :=
         match v with
-        | vstamp vs s => vty (unstamp_vstamp g vs s)
+        | vstamp vs s => unstamp_vstamp g vs s
         | vabs t => vabs (unstamp_tm g t)
         | vty T => vty (unstamp_ty g T)
         | vnat _ => v
@@ -292,72 +293,251 @@ Section translation.
         end
     in go T.
 
-  (* XXX: Not enough, we must also require that e2 contains no concrete types. *)
-  Definition stamps_tm e1 g e2 := e1 = unstamp_tm g e2.
-  Definition stamps_vl v1 g v2 := v1 = unstamp_vl g v2.
-  Definition stamps_ty T1 g T2 := T1 = unstamp_ty g T2.
+  Section fold.
+    Record Traversal {travStateT: Type} {resT: Type} :=
+      {
+        upS: travStateT → travStateT;
+        varP: travStateT → nat → resT;
+        vtyP: travStateT → ty → resT → resT;
+        vstampP: travStateT → vls → list resT → stamp → resT;
+        base: resT;
+        op: resT → resT → resT;
+      }.
+    Global Arguments Traversal _ _: clear implicits.
+    Context `{trav: Traversal travStateT resT}.
+    Local Definition opP := trav.(op).
+    Infix "++" := opP.
+
+    Fixpoint traverse_vl (ts: travStateT) v: resT :=
+      match v with
+      | var_vl i => trav.(varP) ts i
+      | vabs t => traverse_tm (trav.(upS) ts) t
+      | vnat _ => trav.(base)
+      | vty T => trav.(vtyP) ts T (traverse_ty ts T)
+      | vstamp vs s => trav.(vstampP) ts vs (map (traverse_vl ts) vs) s
+      end
+    with
+    traverse_tm (ts: travStateT) e: resT :=
+      match e with
+      | tv v => traverse_vl ts v
+      | tapp t1 t2 => traverse_tm ts t1 ++ traverse_tm ts t2
+      | tskip t => traverse_tm ts t
+      end
+    with
+    traverse_ty (ts: travStateT) T: resT :=
+      match T with
+      | TAll T1 T2 => traverse_ty ts T1 ++ traverse_ty (trav.(upS) ts) T2
+      | TTMem T1 T2 => traverse_ty ts T1 ++ traverse_ty ts T2
+      | TSel v => traverse_vl ts v
+      | TNat => trav.(base)
+      end.
+  End fold.
+
+  Definition is_unstamped_trav: Traversal unit Prop :=
+    {|
+      upS := id;
+      varP := λ s n, True;
+      vtyP := λ s T resT, resT;
+      vstampP := λ s vs ressVs s, False;
+      base := True;
+      op := and
+    |}.
+  Arguments traverse_tm {_} {_} _ _ _: assert.
+  Arguments traverse_ty {_} {_} _ _ _: assert.
+  Arguments traverse_vl {_} {_} _ _ _: assert.
+  Definition is_unstamped_tm := traverse_tm is_unstamped_trav ().
+  Definition is_unstamped_vl := traverse_vl is_unstamped_trav ().
+  Definition is_unstamped_ty := traverse_ty is_unstamped_trav ().
+  Check (is_unstamped_tm: tm → Prop).
+
+  Program Definition is_stamped_trav: Traversal (nat * stys) Prop :=
+    {|
+      upS := λ '(n, g), (S n, g);
+      varP := λ ts n, True;
+      vtyP := λ ts T resT, False;
+      vstampP := λ '(n, g) vs ressVs s, length vs = n ∧ ∃ T, g !! s = Some T ∧ nclosed T n;
+      base := True;
+      op := and
+    |}.
+  (* Beware, the above cannot check that the looked-up types are stamped. Check that separately! *)
+  Definition is_stamped_tm := uncurry (traverse_tm is_stamped_trav).
+  Definition is_stamped_vl := uncurry (traverse_vl is_stamped_trav).
+  Definition is_stamped_ty := uncurry (traverse_ty is_stamped_trav).
+  Check (is_stamped_tm: nat → stys → tm → Prop).
+
+  Definition is_stamped_gmap g: Prop := ∀ s T, g !! s = Some T → ∃ n, is_stamped_ty n g T.
+
+  Definition stamps_tm n e__u g e__s := unstamp_tm g e__s = e__u ∧ is_unstamped_tm e__u ∧ is_stamped_tm n g e__s.
+  Definition stamps_vl n v__u g v__s := unstamp_vl g v__s = v__u ∧ is_unstamped_vl v__u ∧ is_stamped_vl n g v__s.
+  Definition stamps_ty n T__u g T__s := unstamp_ty g T__s = T__u ∧ is_unstamped_ty T__u ∧ is_stamped_ty n g T__s.
 
   (** This lemma suggests this definition is problematic: we don't want empty environments to work.
       They'd fail later lemmas but this is annoying.
       Bigger problem: we should also translate T before storing it in the map! Or after? *)
-  Lemma exists_stamped_vty_bad T g: ∃ v' g', stamps_vl (vty T) g' v' ∧ g ⊆ g'.
+  Lemma exists_stamped_vty T n g: is_unstamped_ty T → nclosed T n → ∃ v' g', stamps_vl n (vty T) g' v' ∧ g ⊆ g'.
   Proof.
-    pose proof (fresh_stamp_strong g T) as [s []].
-    exists (vstamp (idsσ 0) s); rewrite /stamps_vl /unstamp_vl /=; asimpl.
-    exists (<[s:=T]> g); by rewrite lookup_insert /=.
-  Qed.
-
-  Lemma exists_stamped_vty T n g: nclosed T n → ∃ v' g', stamps_vl (vty T) g' v' ∧ g ⊆ g'.
-  Proof.
+    intros Hunst Hcl.
     pose proof (fresh_stamp_strong g T) as [s []].
     exists (vstamp (idsσ n) s); rewrite /stamps_vl /unstamp_vl /=; asimpl.
-    exists (<[s:=T]> g); by rewrite lookup_insert closed_subst_idsρ /=.
+    Require Import DSub.synLemmas.
+    exists (<[s:=T]> g); rewrite lookup_insert /= closed_subst_idsρ // length_idsσ.
+    repeat split; eauto.
   Qed.
 
-  (** Only true for really stamped values. *)
-  Lemma unstamp_mono_tm g1 g2 t: g1 ⊆ g2 → (unstamp_tm g1 t) = (unstamp_tm g2 t). Admitted.
-  Lemma unstamp_mono_vl g1 g2 v: g1 ⊆ g2 → (unstamp_vl g1 v) = (unstamp_vl g2 v). Admitted.
-  Lemma unstamp_mono_ty g1 g2 T: g1 ⊆ g2 → (unstamp_ty g1 T) = (unstamp_ty g2 T). Admitted.
+  (* Lemma exists_stamped_vty_bad T g (n: nat): is_unstamped_ty T → ∃ v' g', stamps_vl 0 (vty T) g' v' ∧ g ⊆ g'. *)
+  (* Proof. *)
+  (*   pose proof (fresh_stamp_strong g T) as [s []]. *)
+  (*   exists (vstamp (idsσ 0) s); rewrite /stamps_vl /unstamp_vl /=; asimpl. *)
+  (*   exists (<[s:=T]> g); rewrite lookup_insert //=; repeat esplit; eauto. *)
+  (* Fail Qed. *)
+  (* Abort. *)
+  Lemma not_stamped_vty g n T:
+    is_stamped_vl n g (vty T) → False.
+  Proof. trivial. Qed.
 
-  (* The statement isn't quite right yet. This only works for properly
-     translated values, and we don't yethave the correct definition. *)
-  Lemma
-    exists_stamped_vl t g: ∃ t' g', stamps_vl t g' t' ∧ g ⊆ g'
-    with
-    exists_stamped_tm t g: ∃ t' g', stamps_tm t g' t' ∧ g ⊆ g'
-    with
-    exists_stamped_ty t g: ∃ t' g', stamps_ty t g' t' ∧ g ⊆ g'.
+  Lemma is_stamped_vty_mono g1 g2 n T:
+    g1 ⊆ g2 →
+    is_stamped_vl n g1 (vty T) →
+    is_stamped_vl n g2 (vty T).
+  Proof. intros; exfalso. by eapply not_stamped_vty. Qed.
+
+  Lemma is_stamped_vstamp_mono g1 g2 n s vs:
+    g1 ⊆ g2 →
+    is_stamped_vl n g1 (vstamp vs s) →
+    is_stamped_vl n g2 (vstamp vs s).
   Proof.
-    all: destruct t eqn:?; rewrite ?/stamps_tm ?/stamps_vl ?/stamps_ty; cbn.
-    all: try by (exists t; exists g; subst; cbn).
-    all: try match goal with
-      | H : context [vstamp _] |- _ => fail 1
-      | H : context [vty _] |- _ => fail 1
-      | H : ?t = ?c ?t1 ?t2 |- _ =>
-        (pose proof (exists_stamped_tm t0_1 g) as (t0_1' & g1 & Hre1 & Hs1) ||
-        pose proof (exists_stamped_vl t0_1 g) as (t0_1' & g1 & Hre1 & Hs1) ||
-        pose proof (exists_stamped_ty t0_1 g) as (t0_1' & g1 & Hre1 & Hs1));
-        (pose proof (exists_stamped_tm t0_2 g1) as (t0_2' & g2 & Hre2 & Hs2) ||
-        pose proof (exists_stamped_vl t0_2 g1) as (t0_2' & g2 & Hre2 & Hs2) ||
-        pose proof (exists_stamped_ty t0_2 g1) as (t0_2' & g2 & Hre2 & Hs2));
-          rewrite Hre1 Hre2 ?(unstamp_mono_tm g1 g2) ?(unstamp_mono_vl g1 g2) ?(unstamp_mono_ty g1 g2) //;
-            try (exists (c t0_1' t0_2'); exists g2=>/=; split; by [f_equiv | destruct t0_1'; destruct t0_2' | simplify_order])
-      | H : ?t = ?c ?t0_1 |- _ =>
-        (pose proof (exists_stamped_tm t0_1 g) as (t0_1' & g1 & Hre1 & Hs1) ||
-        pose proof (exists_stamped_vl t0_1 g) as (t0_1' & g1 & Hre1 & Hs1) ||
-        pose proof (exists_stamped_ty t0_1 g) as (t0_1' & g1 & Hre1 & Hs1));
-          rewrite Hre1;
-            try (exists (c t0_1'); exists g1=>/=; by [f_equiv | destruct t0_1'])
-      end.
-    eapply exists_stamped_vty_bad.
-    (* We should make this impossible. *)
-    admit.
+    (* intros Hg (Hl & T & Hlook & Hcl). *)
+    cbn; intros; ev.
+    repeat esplit => //. by eapply map_subseteq_spec.
+  Qed.
 
-    (* pose proof (exists_stamped_vl v) as (v' & g3 & Hre3 & Hs3). *)
-    (* rewrite Hre3 ?(unstamp_mono_ty g2 g3) //. *)
-    (* exists (TSelA v' t0_1' t0_2'). exists g3. *)
-    (* split; try by [cbn; f_equiv; destruct t0_1'; destruct t0_2' | simplify_order]. *)
+  Arguments is_stamped_vl _ _ !_ /.
+  Arguments is_stamped_ty _ _ !_ /.
+  Arguments is_stamped_tm _ _ !_ /.
+  Arguments prod_uncurry _ _ _ /.
+  Arguments traverse_vl _ _ _: simpl nomatch.
+  Arguments traverse_tm _ _ _: simpl nomatch.
+  Arguments traverse_ty _ _ _: simpl nomatch.
+
+  Lemma
+    is_stamped_mono_tm g1 g2 n e__s:
+    g1 ⊆ g2 →
+    is_stamped_tm n g1 e__s →
+    is_stamped_tm n g2 e__s
+  with
+  is_stamped_mono_vl g1 g2 n v__s:
+    g1 ⊆ g2 →
+    is_stamped_vl n g1 v__s →
+    is_stamped_vl n g2 v__s
+  with
+  is_stamped_mono_ty g1 g2 n T__s:
+    g1 ⊆ g2 →
+    is_stamped_ty n g1 T__s →
+    is_stamped_ty n g2 T__s.
+  Proof.
+    Ltac induct n t__s := intros Hg; revert n; induction t__s; intros n0 Hs; cbn in Hs |- *.
+    - induct n e__s; ev; repeat split_and; by eapply is_stamped_mono_vl || eauto.
+    - induct n v__s; by eapply is_stamped_vstamp_mono || eapply is_stamped_mono_tm || eauto.
+    - induct n T__s; ev; repeat split_and; by eapply is_stamped_mono_vl || eauto || apply IHT__s2.
+  Qed.
+  (* That worked, but a mutual induction principle might be more robust... however, beware the lists!
+     Write it by hand? *)
+
+  Lemma stamps_vty_mono g1 g2 n T v__s:
+    g1 ⊆ g2 →
+    stamps_vl n (vty T) g1 v__s →
+    stamps_vl n (vty T) g2 v__s.
+  Proof.
+    intros Hg (Huns & Hu & Hs).
+    destruct v__s; cbn in *; try solve [inversion Huns | inversion Hs].
+    repeat (split => //; try by eapply is_stamped_mono_vl); cbn.
+    move: Hs Huns => [_] [T'] [Heq1 _] /=.
+    rewrite Heq1 /= => Huns.
+    assert (g2 !! s = Some T') as Heq2. by eapply map_subseteq_spec.
+    rewrite Heq2 //=.
+  Qed.
+
+  Lemma stamps_unstamp_mono_tm g1 g2 n e__u e__s: g1 ⊆ g2 →
+                                     stamps_tm n e__u g1 e__s →
+                                     unstamp_tm g2 e__s = e__u
+  with stamps_unstamp_mono_vl g1 g2 n v__u v__s: g1 ⊆ g2 →
+                                    stamps_vl n v__u g1 v__s →
+                                    unstamp_vl g2 v__s = v__u
+  with stamps_unstamp_mono_ty g1 g2 n T__u T__s: g1 ⊆ g2 →
+                                    stamps_ty n T__u g1 T__s →
+                                    unstamp_ty g2 T__s = T__u.
+  Proof.
+    all: rewrite /stamps_ty /stamps_vl /stamps_tm;
+      intros Hg (Hus & Hu & Hs).
+    -
+      revert n e__u Hs Hu Hus. induction e__s; intros; cbn in Hus |- *;
+        cbn; f_equal; try by subst; f_equal; eapply (stamps_unstamp_mono_vl _ _ _ _ v).
+      cbn in *. subst; f_equal.
+      specialize (IHe__s1 n (unstamp_tm g1 e__s1)).
+      remember (unstamp_tm g1 e__s1) as e eqn:Heqe.
+      unfold unstamp_tm in Heqe. cbv fix in Heqe.
+      cbn in Heqe.
+      unfold unstamp_tm.
+      (* rewrite -IHe__s1. *)
+      (* eapply IHe__s1. *)
+  Abort.
+
+  Lemma stamps_mono_tm g1 g2 n e__u e__s: g1 ⊆ g2 →
+                                     stamps_tm n e__u g1 e__s →
+                                     stamps_tm n e__u g2 e__s
+  with stamps_mono_vl g1 g2 n v__u v__s: g1 ⊆ g2 →
+                                    stamps_vl n v__u g1 v__s →
+                                    stamps_vl n v__u g2 v__s
+  with stamps_mono_ty g1 g2 n T__u T__s: g1 ⊆ g2 →
+                                    stamps_ty n T__u g1 T__s →
+                                    stamps_ty n T__u g2 T__s.
+  Proof.
+    all: rewrite /stamps_ty /stamps_vl /stamps_tm;
+      intros Hg (Hus & Hu & Hs).
+    - revert n Hs; induction e__s => n Hs; cbn in Hus |- *.
+    all: repeat (split => //; try eauto using is_stamped_mono_tm, is_stamped_mono_vl, is_stamped_mono_ty).
+    destruct e__u.
   Admitted.
+
+  (* (* The statement isn't quite right yet. This only works for properly *)
+  (*    translated values, and we don't yethave the correct definition. *) *)
+  (* Lemma *)
+  (*   exists_stamped_vl t g: ∃ t' g', stamps_vl t g' t' ∧ g ⊆ g' *)
+  (*   with *)
+  (*   exists_stamped_tm t g: ∃ t' g', stamps_tm t g' t' ∧ g ⊆ g' *)
+  (*   with *)
+  (*   exists_stamped_ty t g: ∃ t' g', stamps_ty t g' t' ∧ g ⊆ g'. *)
+  (* Proof. *)
+  (*   all: destruct t eqn:?; rewrite ?/stamps_tm ?/stamps_vl ?/stamps_ty; cbn. *)
+  (*   all: try by (exists t; exists g; subst; cbn). *)
+  (*   all: try match goal with *)
+  (*     | H : context [vstamp _] |- _ => fail 1 *)
+  (*     | H : context [vty _] |- _ => fail 1 *)
+  (*     | H : ?t = ?c ?t1 ?t2 |- _ => *)
+  (*       (pose proof (exists_stamped_tm t0_1 g) as (t0_1' & g1 & Hre1 & Hs1) || *)
+  (*       pose proof (exists_stamped_vl t0_1 g) as (t0_1' & g1 & Hre1 & Hs1) || *)
+  (*       pose proof (exists_stamped_ty t0_1 g) as (t0_1' & g1 & Hre1 & Hs1)); *)
+  (*       (pose proof (exists_stamped_tm t0_2 g1) as (t0_2' & g2 & Hre2 & Hs2) || *)
+  (*       pose proof (exists_stamped_vl t0_2 g1) as (t0_2' & g2 & Hre2 & Hs2) || *)
+  (*       pose proof (exists_stamped_ty t0_2 g1) as (t0_2' & g2 & Hre2 & Hs2)); *)
+  (*         rewrite Hre1 Hre2 ?(unstamp_mono_tm g1 g2) ?(unstamp_mono_vl g1 g2) ?(unstamp_mono_ty g1 g2) //; *)
+  (*           try (exists (c t0_1' t0_2'); exists g2=>/=; split; by [f_equiv | destruct t0_1'; destruct t0_2' | simplify_order]) *)
+  (*     | H : ?t = ?c ?t0_1 |- _ => *)
+  (*       (pose proof (exists_stamped_tm t0_1 g) as (t0_1' & g1 & Hre1 & Hs1) || *)
+  (*       pose proof (exists_stamped_vl t0_1 g) as (t0_1' & g1 & Hre1 & Hs1) || *)
+  (*       pose proof (exists_stamped_ty t0_1 g) as (t0_1' & g1 & Hre1 & Hs1)); *)
+  (*         rewrite Hre1; *)
+  (*           try (exists (c t0_1'); exists g1=>/=; by [f_equiv | destruct t0_1']) *)
+  (*     end. *)
+  (*   eapply exists_stamped_vty_bad. *)
+  (*   (* We should make this impossible. *) *)
+  (*   admit. *)
+
+  (*   (* pose proof (exists_stamped_vl v) as (v' & g3 & Hre3 & Hs3). *) *)
+  (*   (* rewrite Hre3 ?(unstamp_mono_ty g2 g3) //. *) *)
+  (*   (* exists (TSelA v' t0_1' t0_2'). exists g3. *) *)
+  (*   (* split; try by [cbn; f_equiv; destruct t0_1'; destruct t0_2' | simplify_order]. *) *)
+  (* Admitted. *)
 
   Fixpoint t_tm n g (t1 t2: tm) {struct t1}: Prop :=
     match (t1, t2) with
@@ -377,7 +557,7 @@ Section translation.
     | (vty T1, vstamp vs s) =>
       (* Needn't we also check that the contents of T1 are syntactic? *)
       nclosed T1 n ∧
-      T1 = unstamp_vstamp g vs s
+      vty T1 = unstamp_vstamp g vs s
     | _ => False
     end.
   Fixpoint t_ty n g (T1 T2: ty) {struct T1}: Prop :=
